progres

Lampe/Lampe/Assignable/Basic.lean
@@ -7,11 +7,84 @@ open Lampe
 
 namespace Lampe.Assignable
 
-def AssignableWithState {tp} (p : Prime) (Γ : Env) (e : Expr (Tp.denote p) tp) (preState postState : State p) (result : tp.denote p) :=
-  ¬Omni p Γ preState e (fun r => r ≠ (postState, result))
+structure CState (p : Prime) where
+  vals : Array (AnyValue p)
+  lambdas : Array (Lambda (Tp.denote p))
+
+instance : Inhabited (CState p) where
+  default := ⟨default, default⟩
+
+theorem CState.default_def : default = @CState.mk p #[] #[] := rfl
+
+def CState.toState (self : CState p) : State p :=
+  State.mk
+    (self.vals.toList.zipIdx.map (fun (v, i) => Sigma.mk (Ref.mk i) v) |>.toFinmap)
+    (self.lambdas.toList.zipIdx.map (fun (l, i) => Sigma.mk (Ref.mk i) l) |>.toFinmap)
+
+def CState.ref {p : Prime} (self : CState p) {tp} (v : Tp.denote p tp) : (Ref × CState p) :=
+  (Ref.mk self.vals.size, { self with vals := self.vals.push ⟨tp, v⟩ })
+
+def CState.lam {p : Prime} (self : CState p) {inTps outTp} (body : HList (Tp.denote p) inTps → Expr (Tp.denote p) outTp) : (Ref × CState p) :=
+  (Ref.mk self.lambdas.size, { self with lambdas := self.lambdas.push ⟨inTps, outTp, body⟩ })
+
+theorem CState.ref_toState_eq_toState_insert {v : Tp.denote p tp}:
+    (CState.ref self v).2.toState = self.toState.insertVal (CState.ref self v).1 ⟨tp, v⟩ := by
+  rw [State.eq_constructor]
+  congr 1
+  simp only [toState, ref, Array.toList_push, State.insertVal]
+  apply Finmap.ext_lookup
+  intro x
+  by_cases h : x = Ref.mk self.vals.size
+  · cases h
+    simp only [List.zipIdx_append, zero_add, List.zipIdx_cons, List.zipIdx_nil,
+      List.map_append, List.map_cons, List.map_nil, Finmap.dlookup_list_toFinmap,
+      List.dlookup_append, List.dlookup_cons_eq, Option.or_some, Finmap.lookup_insert,
+      Option.some.injEq]
+    have : (List.dlookup (Ref.mk self.vals.size) (List.map (fun x ↦ (⟨{ val := x.2 }, x.1⟩ : Sigma (fun _ => AnyValue p))) self.vals.toList.zipIdx)) = none := by
+      rw [List.dlookup_eq_none]
+      simp only [List.keys, List.map_map, List.mem_map, Function.comp_apply, Ref.mk.injEq,
+        Prod.exists, exists_eq_right, not_exists]
+      intro _ hp
+      have := List.mem_zipIdx hp
+      have := this.2.1
+      simp at this
+    simp [this]
+  · simp [h, List.zipIdx_append, List.dlookup_append]
+
+theorem CState.lam_toState_eq_toState_insert {body : HList (Tp.denote p) inTps → Expr (Tp.denote p) outTp}:
+    (CState.lam self body).2.toState = self.toState.insertLam (CState.lam self body).1 ⟨inTps, outTp, body⟩ := by
+  rw [State.eq_constructor]
+  congr 1
+  simp only [toState, lam, Array.toList_push, State.insertLam]
+  apply Finmap.ext_lookup
+  intro x
+  by_cases h : x = Ref.mk self.lambdas.size
+  · cases h
+    simp only [List.zipIdx_append, zero_add, List.zipIdx_cons, List.zipIdx_nil,
+      List.map_append, List.map_cons, List.map_nil, Finmap.dlookup_list_toFinmap,
+      List.dlookup_append, List.dlookup_cons_eq, Option.or_some, Finmap.lookup_insert,
+      Option.some.injEq]
+    have : (List.dlookup (Ref.mk self.lambdas.size) (List.map (fun x ↦ (⟨{ val := x.2 }, x.1⟩ : Sigma (fun _ => Lambda (Tp.denote p)))) self.lambdas.toList.zipIdx)) = none := by
+      rw [List.dlookup_eq_none]
+      simp only [List.keys, List.map_map, List.mem_map, Function.comp_apply, Ref.mk.injEq,
+        Prod.exists, exists_eq_right, not_exists]
+      intro _ hp
+      have := List.mem_zipIdx hp
+      have := this.2.1
+      simp at this
+    simp [this]
+  · simp [h, List.zipIdx_append, List.dlookup_append]
+
+theorem CState.toState_lookup_eq_getElem {self : CState p} {ref : Ref}:
+    (CState.toState self).vals.lookup ref = self.vals[ref.val]? := by
+  sorry
+
+
+def AssignableWithState {tp} (p : Prime) (Γ : Env) (e : Expr (Tp.denote p) tp) (preState postState : CState p) (result : tp.denote p) :=
+  ¬Omni p Γ preState.toState e (fun r => r ≠ (postState.toState, result))
 
 def AssignableMain {tp} (p : Prime) (Γ : Env) (e : Expr (Tp.denote p) tp) (result : tp.denote p) :=
-  ∃postState, AssignableWithState p Γ e (State.mk default default) postState result
+  ∃postState, AssignableWithState p Γ e  default postState result
 
 theorem AssignableWithState.var:
     AssignableWithState p Γ (.var v) state state v := by
@@ -65,6 +138,12 @@ theorem AssignableWithState.fieldLit:
   cases hp
   contradiction
 
+theorem AssignableWithState.litU_intro:
+    AssignableWithState p Γ (Expr.litNum (.u s) n) state state n := by
+  intro hp
+  cases hp
+  contradiction
+
 theorem AssignableWithState.genericPureBuiltin_intro {A} {a : A}
     {sgn : A → List Tp × Tp}
     {desc : {p : Prime}
@@ -108,8 +187,79 @@ theorem AssignableWithState.mkSlice_intro:
   · simp
   · simp
 
--- theorem AssignableWithState.ref_intro
+theorem AssignableWithState.sliceLen_intro:
+    AssignableWithState p env
+      (Expr.callBuiltin [Tp.slice tp] (.u 32) Builtin.arrayLen h![slice])
+      st st slice.length := by
+  apply AssignableWithState.genericPureBuiltin_intro (a := Builtin.ArrayLenCase.slice tp)
 
+theorem AssignableWithState.ref_intro {tp} {v : Tp.denote p tp}:
+    AssignableWithState p Γ (Expr.ref v) state (state.ref v).2 (state.ref v).1 := by
+  intro hp
+  cases hp
+  rename_i hp
+  cases hp
+  rename_i hp
+  apply hp (state.ref v).1
+  · cases state
+    simp only [CState.toState, CState.ref, Finmap.mem_list_toFinmap, List.mem_map, Sigma.mk.injEq,
+      Ref.mk.injEq, heq_eq_eq, Prod.exists, existsAndEq, true_and, exists_eq_right, not_exists]
+    rw [Array.size_eq_length_toList]
+    intro
+    intro h
+    have := (List.mem_zipIdx h).2.1
+    simp at this
+  · simp only [Option.map_some, CState.ref_toState_eq_toState_insert, Option.some.injEq,
+    Prod.mk.injEq, State.eq_constructor, and_true]
+    congr 1
+
+theorem AssignableWithState.lam_intro:
+    AssignableWithState p Γ (Expr.lam argTps outTp b) state (state.lam b).2 (FuncRef.lambda (state.lam b).1) := by
+  intro hp
+  cases hp
+  rename_i hp
+  apply hp (state.lam b).1
+  · cases state
+    simp only [CState.toState, CState.lam, Finmap.mem_list_toFinmap, List.mem_map, Sigma.mk.injEq,
+      Ref.mk.injEq, heq_eq_eq, Prod.exists, existsAndEq, true_and, exists_eq_right, not_exists]
+    rw [Array.size_eq_length_toList]
+    intro
+    intro h
+    have := (List.mem_zipIdx h).2.1
+    simp at this
+  · simp only [Option.map_some, CState.lam_toState_eq_toState_insert, Option.some.injEq,
+    Prod.mk.injEq, State.eq_constructor, and_true]
+    congr 1
+
+theorem AssignableWithState.readRef_intro:
+    (h_ix : ix.val < pre.vals.size) →
+    (h_tp : (pre.vals[ix.val]'h_ix).1 = tp) →
+    AssignableWithState p Γ (Expr.readRef ix) pre pre (h_tp ▸ (pre.vals[ix.val]'h_ix).2) := by
+  intro h_ix h_tp
+  intro hp
+  cases hp
+  rename_i hp
+  cases hp
+  simp_all [mapToValHeapCondition, CState.toState_lookup_eq_getElem]
+  rename pre.vals[_] = _ => hp
+  generalize h: pre.vals[ix.val]'h_ix = x
+  apply_assumption
+  rename tp.denote p => v
+  have h_tp' := h_tp
+  rw [h] at h_tp'
+  have : h_tp ▸ pre.vals[ix.val].snd = h_tp' ▸ x.snd := by
+    cases h
+    rfl
+  rw [this]
+  rw [h] at hp
+  cases hp
+  rfl
+
+theorem AssignableWithState.fn_intro:
+    AssignableWithState p Γ (Expr.fn _ _ r) pre pre r := by
+  intro hp
+  cases hp
+  simp_all
 
 noir_def std::slice::for_each<T: Type, Env: Type>(self: Slice<T>, f: λ(T) -> Unit) -> Unit := {
   let ζi0 = self;
@@ -137,10 +287,20 @@ noir_def std::slice::test::for_each_example<>() -> Unit := {
 
 def env := Env.mk [«std::slice::for_each», «std::slice::test::for_each_example»] []
 
+syntax "norm": tactic
+macro_rules | `(tactic|norm) => `(tactic
+  | try simp only [CState.ref, CState.default_def,
+    List.size_toArray, List.length_nil, List.length_cons, HList.toList,
+    List.push_toArray, List.nil_append])
+
 partial def solve (goal : MVarId): TacticM (List MVarId) := do
+  let [goal] ← evalTacticAt (← `(tactic| norm)) goal
+    | throwError "Failed to simplify goal"
   let target ← goal.instantiateMVarsInType
   let_expr AssignableWithState tp p Γ e pre post res ← target
     | throwError "Goal is not of the form AssignableWithState p Γ e pre post res"
+  let target := mkAppN (.const ``AssignableWithState []) #[tp, p, Γ, e, pre, post, res]
+  let goal ← goal.change target
   match_expr e with
   | Expr.letIn _ _ _ e b =>
     let eGoal :: bGoal :: impls ← goal.apply (.const ``AssignableWithState.letIn [])
@@ -148,27 +308,63 @@ partial def solve (goal : MVarId): TacticM (List MVarId) := do
     let eGoals ← try solve eGoal catch _ => return [eGoal, bGoal] ++ impls
     let bGoals ← try solve bGoal catch _ => return eGoals ++ [bGoal] ++ impls
     return eGoals ++ bGoals ++ impls
-  | Expr.litNum _ tp n => match_expr tp with
+  | Expr.var _ _ _ =>
+    let impl ← goal.apply (.const ``AssignableWithState.var [])
+    return impl
+  | Expr.litNum _ tp _ => match_expr tp with
     | Tp.field =>
       let impl ← goal.apply (.const ``AssignableWithState.fieldLit [])
       return impl
+    | Tp.u _ =>
+      let impl ← goal.apply (.const ``AssignableWithState.litU_intro [])
+      return impl
     | _ => throwError "No applicable rules"
-  | Expr.callBuiltin _ _ _ b _ =>
+  | Expr.fn _ _ _ _ =>
+    let impl ← goal.apply (.const ``AssignableWithState.fn_intro [])
+    return impl
+  | Expr.lam _ _ _ _ =>
+    -- return [goal]
+    let impl ← goal.apply (.const ``AssignableWithState.lam_intro [])
+    return impl
+  | Expr.callBuiltin _ aTps _ b _ =>
     match_expr b with
     | Builtin.mkSlice =>
       let impl ← goal.apply (.const ``AssignableWithState.mkSlice_intro [])
       return impl
+    | Builtin.ref =>
+      let impl ← goal.apply (.const ``AssignableWithState.ref_intro [])
+      return impl
+    | Builtin.arrayLen =>
+      let_expr List.cons _ tp _ ← aTps
+        | throwError "arrayLen should have one argument"
+      match_expr tp with
+      | Tp.slice _ => sorry
+      | Tp.array _ _ => sorry
+      | _ => throwError "arrayLen should take a slice or array"
     | _ => throwError "No applicable rules"
+  | Expr.ref _ _ _ =>
+    let impl ← goal.apply (.const ``AssignableWithState.ref_intro [])
+    return impl
+  | Expr.readRef _ _ _ =>
+    let tp_ok :: ix_ok :: impls ← goal.apply (.const ``AssignableWithState.readRef_intro [])
+      | throwError "Failed to apply readRef_intro"
+    let [] ← evalTacticAt (← `(tactic| norm; decide)) ix_ok
+      | throwError "Failed to prove index is in bounds"
+    tp_ok.refl
+    return impls
   | _ => throwError "No applicable rules"
 
 elab "crush" : tactic => do
   let goal ← getMainGoal
-  replaceMainGoal (← solve goal)
+  replaceMainGoal (←solve goal)
 
 -- unif_hint (p : Prime) (tp tp' : Tp) where
 --   Tp.slice tp' =?= tp
 --   ⊢ Tp.denote p tp =?= List (Tp.denote p tp')
 
+theorem HList.toList_nil : (@HList.nil α β).toList p = [] := by rfl
+
+-- set_option Lampe.pp.Expr true
 
 example : AssignableMain p env («std::slice::test::for_each_example».call h![] h![]) () := by
   apply Exists.intro
@@ -188,5 +384,23 @@ example : AssignableMain p env («std::slice::test::for_each_example».call h![]
   · rfl
   · rfl
   rotate_left
-  simp only
+  crush
+
+  apply AssignableWithState.callDecl
+  · rfl
+  · simp [env]
+    rintro _ (h | h)
+    · apply_fun FunctionDecl.fn at h
+      conv at h => congr <;> whnf
+      cases h
+      rfl
+    · apply_fun FunctionDecl.name at h
+      conv at h => congr <;> whnf
+      simp at h
+  rotate_left
+  · rfl
+  · rfl
+  · rfl
+
+  rotate_right
   crush
